changed the notation of variable and location to not include type

cfrontend/BeePL.v
@@ -16,8 +16,8 @@ Inductive constant : Type :=
 | ConsLong : int64 -> constant
 | ConsUnit : constant.
 
-Record vinfo : Type := mkvar { vname : ident; vtype : BeeTypes.type }.
-Record linfo : Type := mkloc { lname : ident; ltype : BeeTypes.basic_type; lbitfield : bitfield }.
+(*Record vinfo : Type := mkvar { vname : ident; vtype : BeeTypes.basic_type }.*)
+Record linfo : Type := mkloc { lname : ident; (*ltype : BeeTypes.basic_type;*) lbitfield : bitfield }.
 
 Inductive value : Type :=
 | Vunit : value
@@ -66,7 +66,7 @@ match vs, ts with
 | _, _ => False
 end.
 
-Fixpoint extract_types_vinfos (vs : list vinfo) : list BeeTypes.type :=
+(*Fixpoint extract_types_vinfos (vs : list vinfo) : list BeeTypes.basic_type :=
 match vs with 
 | nil => nil
 | v :: vs => v.(vtype) :: extract_types_vinfos vs
@@ -82,7 +82,7 @@ Fixpoint extract_vars_vinfos (vs : list vinfo) : list ident :=
 match vs with 
 | nil => nil
 | v :: vs => v.(vname) :: extract_vars_vinfos vs
-end.
+end.*)
 
 Fixpoint extract_locs_linfos (vs : list linfo) : list ident :=
 match vs with 
@@ -90,17 +90,18 @@ match vs with
 | v :: vs => v.(lname) :: extract_locs_linfos vs
 end.
 
-Fixpoint extract_list_rvtypes (l : list vinfo) : list (ident * BeeTypes.type) :=
+(*Fixpoint extract_list_rvtypes (l : list vinfo) : list (ident * BeeTypes.basic_type) :=
 match l with 
 | nil => nil
 | x :: xs => (x.(vname), x.(vtype)) :: extract_list_rvtypes xs
 end.
 
 Definition eq_vinfo (v1 : vinfo) (v2 : vinfo) : bool :=
-if (v1.(vname) =? v2.(vname))%positive && (eq_type (vtype v1) (vtype v2)) then true else false.
+if (v1.(vname) =? v2.(vname))%positive && (eq_basic_type (vtype v1) (vtype v2)) then true else false.*)
 
+(* add equality over bitfield *)
 Definition eq_linfo (v1 : linfo) (v2 : linfo) : bool :=
-if (v1.(lname) =? v2.(lname))%positive && (eq_basic_type v1.(ltype) v2.(ltype)) then true else false.
+if (v1.(lname) =? v2.(lname))%positive then true else false.
 
 Inductive builtin : Type :=
 | Ref : builtin                             (* allocation : ref t e allocates e of type t 
@@ -140,7 +141,7 @@ end.
    but during evaluation the reductions on heap operations create heaps and use them. *)
 Inductive expr : Type :=
 | Val : value -> type -> expr                                           (* value *) (* rvalue *)
-| Var : vinfo -> expr                                                   (* variable *) (* lvalue *)
+| Var : ident -> type -> expr                                                   (* variable *) (* lvalue *)
 | Const : constant -> type -> expr                                      (* constant *) (* rvalue *)
 | App : expr -> list expr -> type -> expr                               (* function application *) (* rvalue *)
 | Prim : builtin -> list expr -> type -> expr                           (* primitive operations *)
@@ -175,7 +176,7 @@ Definition typeof_expr (e : expr) : BeeTypes.type :=
 match e with 
 | Val v t => t
 (*| Valof e t => t*)
-| Var x => x.(vtype)
+| Var x t => t
 | Const x t => t
 | App e ts t => t
 | Prim b es t => t
@@ -197,8 +198,8 @@ Record function : Type := mkfunction { (*fn_sec: option string; XDP ==> SEC("xdp
                                        fn_return: type;
                                        fn_effect: effect;
                                        fn_callconv: calling_convention;
-                                       fn_args: list vinfo;
-                                       fn_vars: list vinfo;
+                                       fn_args: list (ident * type);
+                                       fn_vars: list (ident * type);
                                        fn_body: expr }.
 
 Inductive fundef : Type :=
@@ -208,7 +209,7 @@ Inductive fundef : Type :=
 (** Type of a function definition. **)
 
 Definition type_of_function (f: function) : type :=
-  Ftype (extract_types_vinfos (fn_args f)) (fn_effect f) (fn_return f).
+  Ftype (unzip2 (fn_args f)) (fn_effect f) (fn_return f).
 
 Definition type_of_fundef (f : fundef) : type :=
 match f with 
@@ -398,26 +399,26 @@ Inductive assign_addr (ty : type) (m : Memory.mem) (addr : Values.block) (ofs : 
    declared in [vars], and associates the variable name with this block. 
    [vm1] and [m1] are the initial local environment and memory state.
    [e2] and [m2] are the final local environment and memory state *) 
-Inductive alloc_variables : vmap -> Memory.mem -> list vinfo -> vmap -> Memory.mem -> Prop :=
+Inductive alloc_variables : vmap -> Memory.mem -> list (ident * type) -> vmap -> Memory.mem -> Prop :=
 | alloc_variables_nil : forall vm hm, 
   alloc_variables vm hm nil vm hm
 | alloc_variables_con : forall e m id ty vars m1 l1 m2 e2,
   Mem.alloc m 0 (sizeof_type ty) = (m1, l1) ->
   alloc_variables (PTree.set id (l1, ty) e) m1 vars e2 m2 ->
-  alloc_variables e m ({| vname := id; vtype := ty |} :: vars) e2 m2.
+  alloc_variables e m ((id, ty) :: vars) e2 m2.
 
 (** Initialization of local variables that are parameters to a function.
   [bind_parameters e m1 params args m2] stores the values [args]
   in the memory blocks corresponding to the variables [params].
   [m1] is the initial memory state and [m2] the final memory state. **)
-Inductive bind_variables  (e: vmap): Memory.mem -> list vinfo -> list value -> Memory.mem -> Prop :=
+Inductive bind_variables  (e: vmap): Memory.mem -> list (ident * type) -> list value -> Memory.mem -> Prop :=
 | bind_variables_nil: forall m,
   bind_variables e m nil nil m
 | bind_variables_cons: forall m id ty params v1 vl v1' b m1 m2,
   PTree.get id e = Some(b, ty) ->
   assign_addr ty m b Ptrofs.zero Full v1 m1 v1' ->
   bind_variables e m1 params vl m2 ->
-  bind_variables e m ({| vname := id; vtype := ty|} :: params) (v1 :: vl) m2.
+  bind_variables e m ((id, ty) :: params) (v1 :: vl) m2.
 
 (** Return the list of blocks in the codomain of [benv], with low and high bounds. **)
 
@@ -429,14 +430,14 @@ Definition blocks_of_env (e: vmap) : list (ident * Z * Z) :=
 
 (* Substitution *)
 Inductive subst : vmap -> Memory.mem -> ident -> value -> expr -> Memory.mem -> expr -> Prop :=
-| var_subst1 : forall vm hm x v y l hm',
-               (x =? y.(vname))%positive = true ->
-               vm!(y.(vname)) = Some (l, y.(vtype)) ->
-               assign_addr y.(vtype) hm l Ptrofs.zero Full v hm' v ->
-               subst vm hm x v (Var y) hm' (Var y)
-| var_subst2 : forall vm hm x v y,
-               (x =? y.(vname))%positive = false -> 
-               subst vm hm x v (Var y) hm (Var y)
+| var_subst1 : forall vm hm x v y t l hm',
+               (x =? y)%positive = true ->
+               vm!y = Some (l, t) ->
+               assign_addr t hm l Ptrofs.zero Full v hm' v ->
+               subst vm hm x v (Var y t) hm' (Var y t)
+| var_subst2 : forall vm hm x v y t,
+               (x =? y)%positive = false -> 
+               subst vm hm x v (Var y t) hm (Var y t)
 | const_subst : forall vm hm x v c t,
                 subst vm hm x v (Const c t) hm (Const c t)
 | app_subst : forall vm hm x v e es t e' hm' hm'' es', (* Fix me *)
@@ -486,7 +487,7 @@ Combined Scheme substs_subst_ind_mut from substs_ind_mut, subst_ind_mut.
 Fixpoint is_simple_expr (e : expr) : bool :=
 match e with 
 | Val v t => true 
-| Var v => true 
+| Var v t => true 
 | Const c t => true
 | App e es t => false 
 | Prim o es t => match o with 
@@ -537,15 +538,15 @@ Variable (vm : vmap).
    We seize this opportunity to define a big-step semantics for simple
    expressions. *) 
 Inductive bsem_expr_slv : Memory.mem -> expr -> linfo -> ptrofs -> Prop :=
-| bsem_var : forall hm x t l h a, 
-              vm!(x.(vname)) = Some (l, Reftype h t a) ->
-              x.(vtype) = Reftype h t a ->
-              bsem_expr_slv hm (Var x) {| lname := l; ltype := t; lbitfield := Full |} Ptrofs.zero
-| bsem_gvar : forall hm x t l h a, 
-              vm!(x.(vname)) = None ->
-              Genv.find_symbol ge x.(vname) = Some l ->
-              x.(vtype) = Reftype h (Bprim t) a ->
-              bsem_expr_slv hm (Var x) {| lname := l; ltype := (Bprim t); lbitfield := Full |} Ptrofs.zero
+| bsem_var : forall hm x t l h t' a, 
+              vm!x = Some (l, Reftype h t' a) ->
+              t = Reftype h t' a ->
+              bsem_expr_slv hm (Var x t) {| lname := l; lbitfield := Full |} Ptrofs.zero
+| bsem_gvar : forall hm x t l h t' a, 
+              vm!x = None ->
+              Genv.find_symbol ge x = Some l ->
+              t = Reftype h (Bprim t') a ->
+              bsem_expr_slv hm (Var x t) {| lname := l; lbitfield := Full |} Ptrofs.zero
 | bsem_addr : forall hm l ofs t,
               bsem_expr_slv hm (Addr l ofs t) l ofs.
 Inductive bsem_expr_srv : Memory.mem -> expr -> value -> Prop :=
@@ -720,8 +721,8 @@ Inductive bestep : state -> state -> Prop :=
                   bsem_expr_srv vm m e v ->
                   transBeePL_type t g = Res ct g' i' ->
                   (gensym ct) = ret fid ->
-                  bind_variables vm m ({| vname := fid; vtype := t|} :: nil) (v :: nil) m' ->
-                  bsem_expr_slv vm m' (Var {| vname := fid; vtype := t |}) l ofs -> 
+                  bind_variables vm m ((fid, t) :: nil) (v :: nil) m' ->
+                  bsem_expr_slv vm m' (Var fid t) l ofs -> 
                   bestep (ExprState f (Prim Ref [:: e] t) k vm m) 
                          (ExprState f (Val (Vloc l.(lname) ofs) t) k vm m') 
 | step_prim_massgn : forall vm f k e1 e2 t ct1 ct2 l ofs m v g1 g2 g3 i i' v' m', 
@@ -892,31 +893,32 @@ Variable (ge : genv).
 Variable (vm : vmap).
 
 Inductive lreduction : expr -> Memory.mem -> expr -> Memory.mem -> Prop :=
-| lred_var_local : forall hm x t l h a,
-                   vm!(x.(vname)) = Some (l, Reftype h (Bprim t) a) ->
-                   x.(vtype) = Reftype h (Bprim t) a ->
-                   lreduction (Var x) hm (Addr {| lname := l; ltype := Bprim t; lbitfield := Full |} Ptrofs.zero (Reftype h (Bprim t) a)) hm
-| lred_var_global : forall hm x t l h a,
-                    vm!(x.(vname)) = None ->
-                    x.(vtype) = Reftype h (Bprim t) a ->
-                    Genv.find_symbol ge x.(vname) = Some l ->
-                    lreduction (Var x) hm (Addr {| lname := l; ltype := Bprim t; lbitfield := Full |} Ptrofs.zero 
-                                           (Reftype h (Bprim t) a)) hm.
+| lred_var_local : forall hm x t l h t' a,
+                   vm!x = Some (l, Reftype h (Bprim t') a) ->
+                   t = Reftype h (Bprim t') a ->
+                   lreduction (Var x t) hm (Addr {| lname := l; lbitfield := Full |} 
+                                            Ptrofs.zero (Reftype h (Bprim t') a)) hm
+| lred_var_global : forall hm x t l h t' a,
+                    vm!x = None ->
+                    t = Reftype h (Bprim t') a ->
+                    Genv.find_symbol ge x = Some l ->
+                    lreduction (Var x t) hm (Addr {| lname := l; lbitfield := Full |} Ptrofs.zero 
+                                             (Reftype h (Bprim t') a)) hm.
 
 Inductive rreduction : expr -> Memory.mem -> expr -> Memory.mem -> Prop :=
 | rred_valof : forall hm t l ofs bf v h a,
                deref_addr ge (Ptype t) hm l ofs bf v ->
                BeeTypes.type_is_volatile (Ptype t) = false ->
-               rreduction (Prim Deref ((Addr {| lname := l; ltype := Bprim t; lbitfield := bf |} ofs (Reftype h (Bprim t) a)) :: nil) (Ptype t)) hm 
+               rreduction (Prim Deref ((Addr {| lname := l; lbitfield := bf |} ofs (Reftype h (Bprim t) a)) :: nil) (Ptype t)) hm 
                (Val v (Ptype t)) hm
 | rred_ref : forall hm t g ct g' i' fid hm' v l ofs h a, 
              transBeePL_type (Ptype t) g = Res ct g' i' ->
              (gensym ct) = ret fid ->
-             bind_variables ge vm hm ({| vname := fid; vtype := Ptype t|} :: nil) (v :: nil) hm' ->
-             lreduction (Var {| vname := fid; vtype := Ptype t |}) hm' 
-                        (Addr {| lname := l; ltype := Bprim t; lbitfield := Full |} Ptrofs.zero (Reftype h (Bprim t) a)) ofs -> 
+             bind_variables ge vm hm ((fid, (Ptype t)) :: nil) (v :: nil) hm' ->
+             lreduction (Var fid (Ptype t)) hm' 
+                        (Addr {| lname := l; lbitfield := Full |} Ptrofs.zero (Reftype h (Bprim t) a)) ofs -> 
              rreduction (Prim Ref [:: (Val v (Ptype t))] (Ptype t)) hm 
-                        (Addr {| lname := l; ltype := Bprim t; lbitfield :=  Full|} Ptrofs.zero (Reftype h (Bprim t) a)) hm'
+                        (Addr {| lname := l; lbitfield :=  Full|} Ptrofs.zero (Reftype h (Bprim t) a)) hm'
 | rred_uop : forall hm v t ct uop v' v'' g g' i',
              transBeePL_type t g = Res ct g' i' ->
              sem_unary_operation uop (transBeePL_value_cvalue v) ct hm = Some v' -> 
@@ -937,7 +939,7 @@ Inductive rreduction : expr -> Memory.mem -> expr -> Memory.mem -> Prop :=
                 transBeePL_type (Ptype tv2) g' = Res ct2 g'' i''->
                 sem_cast (transBeePL_value_cvalue v) ct2 ct1 hm = Some (transBeePL_value_cvalue v') ->
                 assign_addr ge (Ptype t) hm l ofs bf v' hm' v' ->
-                rreduction (Prim Massgn ((Addr {| lname := l; ltype := Bprim t; lbitfield := bf |} ofs (Reftype h (Bprim t) a)) 
+                rreduction (Prim Massgn ((Addr {| lname := l; lbitfield := bf |} ofs (Reftype h (Bprim t) a)) 
                                          :: Val v (Ptype tv2) :: nil) (Ptype t)) hm (Val v' (Ptype t)) hm'
 | rred_bind : forall vm hm x v e2 e2' t t' hm',
               subst ge vm hm x v e2 hm' e2' ->
