cfrontend/BeePL_typesystem.v
@@ -1,6 +1,6 @@
 Require Import String ZArith Coq.FSets.FMapAVL Coq.Structures.OrderedTypeEx.
 Require Import Coq.FSets.FSetProperties Coq.FSets.FMapFacts FMaps FSetAVL Nat PeanoNat.
-Require Import Coq.Arith.EqNat Coq.ZArith.Int Integers AST Maps Coqlib Memory Ctypes Memtype.
+Require Import Coq.Arith.EqNat Coq.ZArith.Int Integers AST Maps Globalenvs Coqlib Memory Ctypes Memtype.
 Require Import BeePL_aux BeePL_mem BeeTypes BeePL BeePL_auxlemmas BeePL_sem BeePL_compiler_proofs.
 From mathcomp Require Import all_ssreflect. 
 
@@ -14,9 +14,8 @@ Inductive type_expr : ty_context -> store_context -> expr -> effect -> type -> P
 | ty_val : forall Gamma Sigma v ef t,
            type_expr Gamma Sigma (Val v t) ef t
 | ty_var : forall Gamma Sigma x t, 
-           PTree.get x.(vname) (extend_context Gamma x.(vname) t) = Some t ->
-           x.(vtype) = t ->
-           type_expr Gamma Sigma (Var x) empty_effect t
+           PTree.get x (extend_context Gamma x (Ptype t)) = Some (Ptype t) ->
+           type_expr Gamma Sigma (Var x (Ptype t)) empty_effect (Ptype t)
 | ty_constint : forall Gamma Sigma t sz s a i,
                 t = (Ptype (Tint sz s a)) ->
                 type_expr Gamma Sigma (Const (ConsInt i) t) empty_effect t
@@ -62,10 +61,10 @@ Inductive type_expr : ty_context -> store_context -> expr -> effect -> type -> P
             type_expr Gamma Sigma (Cond e1 e2 e3 t) (ef1 ++ ef2 ++ ef3) t
 | ty_unit : forall Gamma Sigma,
             type_expr Gamma Sigma (Unit (Ptype Tunit)) empty_effect (Ptype Tunit)
-| ty_addr : forall Gamma Sigma l ofs h t a,
-            PTree.get l.(lname) Sigma = Some l.(ltype) ->
-            t = (Reftype h l.(ltype) a) ->
-            type_expr Gamma Sigma (Addr l ofs t) empty_effect t 
+| ty_addr : forall Gamma Sigma l ofs h t a t',
+            PTree.get l.(lname) Sigma = Some t ->
+            t' = (Reftype h t a) ->
+            type_expr Gamma Sigma (Addr l ofs t') empty_effect t' 
 (* fix me : Run *)
 (* fix me : Hexpr *)
 (*| ty_hexpr : forall Gamma Sigma m e h ef t a, 
@@ -97,18 +96,9 @@ Context (Pts : ty_context -> store_context -> list expr -> effect -> list type -
 Context (Pt : ty_context -> store_context -> expr -> effect -> type -> Prop).
 Context (Htval : forall Gamma Sigma v ef t,
                  Pt Gamma Sigma (Val v t) ef t).
-(*Context (Htvalu : forall Gamma Sigma,
-                  Pt Gamma Sigma (Val Vunit (Ptype Tunit)) empty_effect (Ptype Tunit)).
-Context (Htvali Ty_val_int : forall Gamma Sigma i sz s a,
-                             Pt Gamma Sigma (Val (Vint i) (Ptype (Tint sz s a))) empty_effect (Ptype (Tint sz s a))).
-Context (Htvall : forall Gamma Sigma i s a,
-                  Pt Gamma Sigma (Val (Vint64 i) (Ptype (Tlong s a))) empty_effect (Ptype (Tlong s a))).
-Context (Htvalloc : forall Gamma Sigma h t l ofs a,
-                    Pt Gamma Sigma (Val (Vloc l ofs) (Reftype h (Bprim t) a)) empty_effect (Reftype h (Bprim t) a)). *)
 Context (Htvar : forall Gamma Sigma x t,
-                 PTree.get x.(vname) (extend_context Gamma x.(vname) t) = Some t ->
-                 x.(vtype) = t ->
-                 Pt Gamma Sigma (Var x) empty_effect t).
+                 PTree.get x (extend_context Gamma x (Ptype t)) = Some (Ptype t) ->
+                 Pt Gamma Sigma (Var x (Ptype t)) empty_effect (Ptype t)).
 Context (Htconti : forall Gamma Sigma t sz s i a,
                    t = (Ptype (Tint sz s a)) ->
                    Pt Gamma Sigma (Const (ConsInt i) t) empty_effect t).
@@ -151,10 +141,10 @@ Context (Htcond : forall Gamma Sigma e1 e2 e3 ef1 ef2 ef3 tb t,
                   Pt Gamma Sigma (Cond e1 e2 e3 t) (ef1 ++ ef2 ++ ef3) t).
 Context (Htunit : forall Gamma Sigma, 
                   Pt Gamma Sigma (Unit (Ptype Tunit)) empty_effect (Ptype Tunit)).
-Context (Htloc : forall Gamma Sigma l h t a ofs, 
-                 PTree.get l.(lname) Sigma = Some l.(ltype)  ->
-                 t = (Reftype h l.(ltype) a) ->
-                 Pt Gamma Sigma (Addr l ofs t) empty_effect t). 
+Context (Htloc : forall Gamma Sigma l h t a ofs t', 
+                 PTree.get l.(lname) Sigma = Some t  ->
+                 t' = (Reftype h t a) ->
+                 Pt Gamma Sigma (Addr l ofs t') empty_effect t'). 
 (*Context (Htheap : forall Gamma Sigma m e h ef t a, 
                   Pt Gamma Sigma e ef (Reftype h (Bprim t) a) ->
                   Pt Gamma Sigma (Hexpr m e (Reftype h (Bprim t) a)) ef (Reftype h (Bprim t) a)).*)
@@ -229,7 +219,7 @@ suff : (forall Gamma Sigma es efs ts, type_exprs Gamma Sigma es efs ts ->
   by move: (ih' Gamma Sigma e ef t he ef' t' he').
 apply type_expr_indP => //=.
 + admit. (*by move=> Gamma Sigma v ef t ef' t' ht; inversion ht; subst.*)
-+ move=> Gamma Sigma x t htx ht ef' t' het; subst. by inversion het; subst.
++ move=> Gamma Sigma x t ht ef' t' het; subst. by inversion het; subst.
 + move=> Gamma Sigma t sz s i a ht ef' t' ht'; subst. by inversion ht'; subst.
 + move=> Gamma Sigma t s i a ht ef' t' ht'; subst. by inversion ht'; subst.
 + move=> Gamma Sigma t ht ef' t' ht'; subst. by inversion ht'; subst.
@@ -254,7 +244,7 @@ apply type_expr_indP => //=.
   move: (ih1 ef0 tb0 H5)=> [] h1 h2; subst. move: (ih2 ef4 t' H9)=> [] h1' h2'; subst.
   by move: (ih3 ef5 t' H10)=> [] h1'' h2''; subst.
 + by move=> Gamma Sigma efs' ts' ht; inversion ht; subst.
-+ by move=> Gamma Sigma l h t a ofs hs hl ef' t' ht; inversion ht; subst.
++ by move=> Gamma Sigma l h t a ofs t' hs hl ef' t'' ht; inversion ht; subst.
 + by move=> Gamma Sigma efs' ts' ht; inversion ht; subst.
 move=> Gamma Sigma e es t ef ts efs ih ih' efs' ts' ht; inversion ht; subst.
 move: (ih ef0 t0 H3)=> [] h1 h2; subst. by move: (ih' efs0 ts0 H6)=> [] h1 h2; subst.
@@ -293,17 +283,17 @@ Qed.
    able to substitute [e'] for each of the occurrences of [x] in [e]
    and obtain a new expression that still has type [t]. *)
 Lemma wsubst_preservation : forall Gamma Sigma bge vm hm hm' x t v e ef t' e'', 
-type_expr (extend_context Gamma x.(vname) t) Sigma e ef t' ->
+type_expr (extend_context Gamma x t) Sigma e ef t' ->
 wtypeof_value v (wtype_of_type t) ->
-subst bge vm hm x.(vname) v e hm' e'' ->
+subst bge vm hm x v e hm' e'' ->
 type_expr Gamma Sigma e'' ef t'.
 Proof.
 Admitted.
 
 Lemma subst_preservation : forall Gamma Sigma bge vm hm hm' x t v e ef t' e'', 
-type_expr (extend_context Gamma x.(vname) t) Sigma e ef t' ->
+type_expr (extend_context Gamma x t) Sigma e ef t' ->
 typeof_value v t ->
-subst bge vm hm x.(vname) v e hm' e'' ->
+subst bge vm hm x v e hm' e'' ->
 type_expr Gamma Sigma e'' ef t'.
 Proof.
 Admitted.
@@ -469,48 +459,65 @@ Qed.
 (**** Well formedness ****)
 (** Well-Typed Store **)
 (* A store st is well-typed with respect to a store typing context Sigma if the
-   term at each location l in st has the type at location l in ST *)
-Definition store_well_typed (Sigma : store_context) (vm : vmap) :=
-forall l t, 
-exists v, vm! l = Some(v, (Ptype t)) /\
-PTree.get l Sigma = Some (Bprim t).
+   term at each location l in vm has the type at location l in store typing context
+   and there exists a value in the memory at that location. *)
+Definition store_well_typed (Sigma : store_context) (bge : genv) (vm : vmap) (m : Memory.mem) :=
+(forall l t, 
+ exists l' ofs v, vm! l = Some(l', (Ptype t)) /\
+                  PTree.get l Sigma = Some (Bprim t) /\ 
+                  deref_addr bge (Ptype t) m l' ofs Full v) \/
+(forall l t, vm! l = None /\ 
+             exists l' ofs v, Genv.find_symbol bge l = Some l' /\ 
+                              deref_addr bge t m l' ofs Full v).
 
-(*** Proving theorems related to type system for small step semantics of BeePL *)
+(*** Proving theorems related to type system for small step semantics of BeePL ***)
+
+(* Progress for small step semantics *)
 Lemma progress_ssem_expr_exprs:
 (forall Gamma Sigma es efs ts bge vm m, type_exprs Gamma Sigma es efs ts ->
-                                        store_well_typed Sigma vm ->
+                                        store_well_typed Sigma bge vm m ->
                                         is_values es \/ exists m' vm' es',
                                                         ssem_exprs bge vm m es m' vm' es') /\
 (forall Gamma Sigma e ef t bge vm m, type_expr Gamma Sigma e ef t ->
-                                     store_well_typed Sigma vm ->
+                                     store_well_typed Sigma bge vm m ->
                                      is_value e \/ exists m' vm' e', 
                                                    ssem_expr bge vm m e m' vm' e').
 Proof.
 suff : (forall Gamma Sigma es efs ts, type_exprs Gamma Sigma es efs ts ->
-                                      forall bge vm m, store_well_typed Sigma vm ->
+                                      forall bge vm m, store_well_typed Sigma bge vm m ->
                                                        is_values es \/ exists m' vm' es',
                                                        ssem_exprs bge vm m es m' vm' es') /\
 (forall Gamma Sigma e ef t, type_expr Gamma Sigma e ef t ->
-                            forall bge vm m, store_well_typed Sigma vm ->
+                            forall bge vm m, store_well_typed Sigma bge vm m ->
                                              is_value e \/ exists m' vm' e', 
                                                            ssem_expr bge vm m e m' vm' e').
 + admit.
 apply type_exprs_type_expr_ind_mut=> //=.
 (* val *)
 + move=> Gamma Sigma v ef t bge vm m. by left.
-(* lvar *)
-+ move=> Gamma Sigma v t ht hteq bge vm m hw; subst. right.
-  rewrite /store_well_typed in hw. 
-  exists m. exists vm. eexists. eapply ssem_lvar. + admit.
-  admit. 
-(* gvar *)
-+ admit.
+(* var *)
++ move=> Gamma Sigma v t hteq bge vm m hw; subst. right.
+  rewrite /store_well_typed in hw. case: hw=> hw.
+  (* lvar *)
+  + move:(hw v t)=> [] l [] ofs [] v' [] hvm [] hs hd.
+    exists m. exists vm. exists (Val v' (Ptype t)). eapply ssem_lvar.
+    + by apply hvm. 
+    by apply hd.  
+  (* gvar *)
+  move: (hw v (Ptype t))=> [] hvm [] l' [] ofs [] v' [] hbge hd.
+  exists m. exists vm. exists (Val v' (Ptype t)). apply ssem_gbvar with l' ofs.
+  + by apply hvm.
+  + by apply hbge.
+  by apply hd.
+(* const int *)
++ move=> Gamma Sigma t sz s a i ht bge vm m hw. right.
+  exists m. exists vm. exists (Val (Vint i) t). by apply ssem_consti.
 (* const long *)
-+ admit.
++ move=> Gamma Sigma t s a i ht bge vm m hw. right.
+  exists m. exists vm. exists (Val (Vint64 i) t). by apply ssem_constl.
 (* const uint *)
 + move=> Gamma Sigma t hteq bge vm m. right; subst.
-  exists m. exists vm. exists (Val (Vunit) (Ptype Tunit)).
-  by apply ssem_constu.
+  exists m. exists vm. exists (Val (Vunit) (Ptype Tunit)). by apply ssem_constu.
 (* app *)
 + admit.
 (* ref *)
@@ -680,11 +687,13 @@ apply type_expr_indP => //=.
     move=> i h a he hw. case: v' he hw=> //= i' he hw. by inversion hw.
   move=> es e t he hw. case: v' he hw=> //= i he hw. by inversion hw.
 (* var *)
-+ move=> Gamma Sigma x t ht hteq bge vm m vm' m' v hv. inversion hv; subst.
++ move=> Gamma Sigma x t ht bge vm m vm' m' v hv. inversion hv; subst.
   (* local *)
-  + by have := wderef_addr_val_ty bge (vtype x) m' l ofs Full v H3.
+  + have := wderef_addr_val_ty bge (Ptype t) m' l ofs Full v H7.
+    by case: t ht hv H3 H7=> //=.
   (* global *)
-  + by have := wderef_addr_val_ty bge (vtype x) m' l ofs Full v H4.
+  + have := wderef_addr_val_ty bge (Ptype t) m' l ofs Full v H8.
+    by case: t ht hv H8=> //=.
 (* const int *)
 + move=> Gamma Sigma t sz s i a hteq bge vm m vm' m' v hv. by inversion hv; subst.
 (* const long *)
@@ -730,8 +739,8 @@ apply type_expr_indP => //=.
 (* unit *)
 + move=> Gamma Sigma bge vm m vm' m' v he. by inversion he; subst.
 (* addr *)
-+ move=> Gamma Sigma l h t a ofs hs ht bge vm m vm' m' v he.
-  rewrite ht /=. by inversion he; subst.
++ move=> Gamma Sigma l h t a ofs t' ht hteq bge vm m vm' m' v he.
+  rewrite hteq /=. by inversion he; subst.
 (* nil *)
 + move=> Gamma Sigma bge vm m vm' m' vs hv. by inversion hv; subst.
 (* cons *)
@@ -750,13 +759,11 @@ Variable (benv : vmap).
 Lemma subject_lredcution : forall m e l ofs Gamma Sigma ef t h a,
 bsem_expr_slv bge benv m e l ofs ->
 type_expr Gamma Sigma e ef (Reftype h t a) ->
-l.(ltype) = t.
+PTree.get l.(lname) Sigma = Some t.
 Proof.
 move=> m e l ofs Gamma Sigma ef t h a hl.
 induction hl=> //= ht; subst; inversion ht; subst; symmetry.
-+ rewrite H0 in H5. by case: H5=> h1 h2 h3; subst.
-+ rewrite H1 in H6. by case: H6=> h1 h2 h3; subst.
-by inversion H7; subst. 
+by case: H7=> h1 h2 h3; subst.
 Qed.
 
 Lemma subject_rreduction : forall m e v Gamma Sigma ef t, 
